x86model/Model/ParserTest.v
@@ -10,99 +10,280 @@
 *)
 
 Require Coqlib.
-Require Import Parser.
 Require Import Ascii.
 Require Import String.
 Require Import List.
+Require Import ZArith.
+
+Require ParserArg.
+Import ParserArg.X86_PARSER_ARG.
+Require Import Parser.
+Require Import Bits.
+
 Unset Automatic Introduction.
 Set Implicit Arguments.
 Open Scope char_scope.
+Local Open Scope Z_scope.
 
 
 Require ExtrOcamlString.
 Require ExtrOcamlNatBigInt.
 (*Require ExtrOcamlNatInt.*)
 
-Module TEST_PARSER_ARG.
-  Definition char_p := bool.
-  Definition char_eq := Bool.bool_dec.
 
-  Inductive type : Set := 
-  | Int_t : type.
+Section Grammar1.
 
-  Definition tipe := type.
-  Definition tipe_eq : forall (t1 t2:tipe), {t1=t2} + {t1<>t2}.
-    intros ; decide equality.
-  Defined.
-  Definition tipe_m (t:tipe) := 
-    match t with 
-      | Int_t => nat
+  Definition int_t := User_t Int_t.
+
+  Definition byte_t := User_t Byte_t.
+
+  Definition map t1 t2 (p:grammar t1) (f:interp t1 -> interp t2) : grammar t2 := 
+    @Map t1 t2 f p.
+  Implicit Arguments map [t1 t2].
+
+  Definition seq t1 t2 (p1:grammar t1) (p2:grammar t2) : grammar (Pair_t t1 t2) := 
+    Cat p1 p2.
+
+  Definition alt t (p1 p2:grammar t) : grammar t := 
+    Map _ (fun (x:interp (Sum_t t t)) => match x with inl a => a | inr b => b end) 
+        (Alt p1 p2).
+
+  Infix "$" := seq (right associativity, at level 70).
+  Infix "@" := map (right associativity, at level 75).
+  Infix "|+|" := alt (right associativity, at level 80).
+  Notation "e %% t" := (e : interp t) (at level 80).
+
+  Fixpoint bits_n (n:nat) : type := 
+    match n with 
+      | 0%nat => Unit_t
+      | S n => Pair_t Char_t (bits_n n)
     end.
-End TEST_PARSER_ARG.
 
-Module TEST_PARSER.
-Module T := Parser.Parser(TEST_PARSER_ARG).
-Import TEST_PARSER_ARG.
-Import T.
-Infix "|+|" := Alt_p (right associativity, at level 80).
-Infix "$" := Cat_p (right associativity, at level 70).
-Definition map_p t1 t2 (p:parser t1) (f:result_m t1 -> result_m t2) := @Map_p t1 t2 f p.
-Implicit Arguments map_p [t1 t2].
-Infix "@" := map_p (right associativity, at level 75).
-Definition Plus_p t (p:parser t) := 
-  (Cat_p p (Star_p p)) @ (fun p => ((fst p)::(snd p)): result_m (list_t t)).
-Definition Alts_p t (ps:list (parser t)) := 
-  List.fold_right (@Alt_p t) (Zero_p t) ps.
-Definition int_t := tipe_t Int_t.
-Notation "e %% t" := (e : result_m t) (at level 80).
+  Fixpoint bits (x:string) : grammar (bits_n (String.length x)) := 
+    match x with 
+      | EmptyString => Eps
+      | String c s => 
+        (Cat (Char (if ascii_dec c "0"%char then false else true)) (bits s))
+    end.
 
-Definition one := Char_p true @ (fun _ => 1 %% int_t).
-Definition zero := Char_p false @ (fun _ => 0 %% int_t).
-Definition bit' := zero |+| one.
-Definition bit := Any_p @ (fun c => (if c then 1 else 0) %% int_t).
-Definition nibble := 
-  bit $ bit $ bit $ bit @ 
-  (fun x => match x with 
-              | (b3,(b2,(b1,b0))) => b0 + 2*b1 + 4*b2 + 8*b3
-            end %% int_t).
-Definition byte := 
-  nibble $ nibble @ (fun p => (snd p + (fst p)*256) %% int_t).
+  Fixpoint bits2Z(n:nat)(a:Z) : interp (bits_n n) -> interp int_t := 
+    match n with 
+      | 0%nat => fun _ => a
+      | S n => fun p => bits2Z n (2*a + (if (fst p) then 1 else 0)) (snd p)
+    end.
 
-(* is a parser deterministic for strings up to length n? 
-Definition is_deterministic t (p:parser t) n := 
-  is_determ (snd (parser2regexp p)) 2 (fun n => (match n with 0 => false | _ => true end)::nil) n
-  (fst (parser2regexp p)) (p2r_wf p _).
+  Fixpoint field'(n:nat) : grammar (bits_n n) := 
+    match n with 
+      | 0%nat => Eps
+      | S n => Cat Any (field' n)
+    end.
 
-Lemma is_deterministic_byte : is_deterministic byte 8 = true.
-Proof.
-  auto.
-Qed.
+  Definition bits2int(n:nat)(bs:interp (bits_n n)) : interp int_t := bits2Z n 0 bs.
 
-Definition ambiguous_p := nibble |+| nibble.
+  Definition field(n:nat) := (field' n) @ (bits2int n).
+  Definition byte := (field 8) @ (@Word.repr 7 : _ -> interp byte_t).
 
-Lemma is_deterministic_ambiguous_p : is_deterministic ambiguous_p 4 = false.
-Proof.
-  auto.
-Qed.
-*)
-Fixpoint explode(s:string) : list bool := 
-  match s with 
-    | ""%string => nil
-    | String "0" t => false::(explode t)
-    | String _ t => true::(explode t)
+  Definition listint_t := List_t (User_t Int_t).
+
+  (* g_n consumes 2^n bytes and has 2^(2^n) cases *)
+  Definition g0 := (bits "11111110" |+| bits "11111111")
+                     @ (fun v => (bits2int 8 v) :: nil %% listint_t).
+  Definition g1 := (g0 $ g0) @ (fun p => app (fst p) (snd p) %% listint_t).
+  Definition g2 := (g1 $ g1) @ (fun p => app (fst p) (snd p) %% listint_t).
+  Definition g3 := (g2 $ g2) @ (fun p => app (fst p) (snd p) %% listint_t).
+  Definition g4 := (g3 $ g3) @ (fun p => app (fst p) (snd p) %% listint_t).
+  Definition g5 := (g4 $ g4) @ (fun p => app (fst p) (snd p) %% listint_t).
+  Definition g6 := (g5 $ g5) @ (fun p => app (fst p) (snd p) %% listint_t).
+  Definition g7 := (g6 $ g6) @ (fun p => app (fst p) (snd p) %% listint_t).
+  Definition g8 := (g7 $ g7) @ (fun p => app (fst p) (snd p) %% listint_t).
+  Definition g9 := (g8 $ g8) @ (fun p => app (fst p) (snd p) %% listint_t).
+  Definition g10 := (g9 $ g9) @ (fun p => app (fst p) (snd p) %% listint_t).
+  Definition g11 := (g10 $ g10) @ (fun p => app (fst p) (snd p) %% listint_t).
+  Definition g12 := (g11 $ g11) @ (fun p => app (fst p) (snd p) %% listint_t).
+  Definition g13 := (g12 $ g12) @ (fun p => app (fst p) (snd p) %% listint_t).
+  Definition g14 := (g13 $ g13) @ (fun p => app (fst p) (snd p) %% listint_t).
+  Definition g15 := (g14 $ g14) @ (fun p => app (fst p) (snd p) %% listint_t).
+  Definition g16 := (g15 $ g15) @ (fun p => app (fst p) (snd p) %% listint_t).
+  Definition g17 := (g16 $ g16) @ (fun p => app (fst p) (snd p) %% listint_t).
+  Definition g18 := (g17 $ g17) @ (fun p => app (fst p) (snd p) %% listint_t).
+  Definition g19 := (g18 $ g18) @ (fun p => app (fst p) (snd p) %% listint_t).
+  Definition g20 := (g19 $ g19) @ (fun p => app (fst p) (snd p) %% listint_t).
+
+(* prefix_n consumes 2^n 0xff bytes *)
+Definition prefix0 := bits "11111111" @ (fun v => (bits2int 8 v) :: nil %% listint_t).
+Definition prefix1 := (prefix0 $ prefix0) @ (fun p => app (fst p) (snd p) %% listint_t).
+Definition prefix2 := (prefix1 $ prefix1) @ (fun p => app (fst p) (snd p) %% listint_t).
+Definition prefix3 := (prefix2 $ prefix2) @ (fun p => app (fst p) (snd p) %% listint_t).
+Definition prefix4 := (prefix3 $ prefix3) @ (fun p => app (fst p) (snd p) %% listint_t).
+Definition prefix5 := (prefix4 $ prefix4) @ (fun p => app (fst p) (snd p) %% listint_t).
+Definition prefix6 := (prefix5 $ prefix5) @ (fun p => app (fst p) (snd p) %% listint_t).
+Definition prefix7 := (prefix6 $ prefix6) @ (fun p => app (fst p) (snd p) %% listint_t).
+Definition prefix8 := (prefix7 $ prefix7) @ (fun p => app (fst p) (snd p) %% listint_t).
+Definition prefix9 := (prefix8 $ prefix8) @ (fun p => app (fst p) (snd p) %% listint_t).
+Definition prefix10 := (prefix9 $ prefix9) @ (fun p => app (fst p) (snd p) %% listint_t).
+Definition prefix11 := (prefix10 $ prefix10) @ (fun p => app (fst p) (snd p) %% listint_t).
+Definition prefix12 := (prefix11 $ prefix11) @ (fun p => app (fst p) (snd p) %% listint_t).
+Definition prefix13 := (prefix12 $ prefix12) @ (fun p => app (fst p) (snd p) %% listint_t).
+
+Fixpoint perm (l:list (grammar listint_t)) : list (grammar listint_t) := 
+  match l with
+    | nil => nil
+    | h::t =>
+      ((bits "11111111" $ h) @ (fun p => (bits2int 8 (fst p) :: snd p) %% listint_t)) ::
+      ((bits "11111110" $ h) @ (fun p => (bits2int 8 (fst p) :: snd p) %% listint_t)) ::
+      perm t
   end.
 
-Definition lex t (p:parser t) s := parse p (explode s).
+(* p_n consumes n bytes, each byte can be a 0xff or a 0xfe *)
+Definition p0 := (Eps @ (fun _ => nil %% listint_t)) :: nil.
+Definition p1 := perm p0.
+Definition p2 := perm p1.
+Definition p3 := perm p2.
+Definition p4 := perm p3.
+Definition p5 := perm p4.
+Definition p6 := perm p5.
+Definition p7 := perm p6.
+Definition p8 := perm p7.
+Definition p9 := perm p8.
+Definition p10 := perm p9.
+Definition p11 := perm p10.
+Definition p12 := perm p11.
+Definition p13 := perm p12.
 
-(*
-Opaque result_m.
-Opaque p2r_wf.
-Opaque wf_derivs.
-*)
-Eval simpl in lex (nibble) "011". 
-Eval simpl in explode("1000111").
-Eval simpl in nibble 1.
-End TEST_PARSER.
+  Definition never t : grammar t := Zero t.
+
+  Fixpoint alts0 t (ps:list (grammar t)) : grammar t := 
+    match ps with 
+      | nil => @never t
+      | p::nil => p
+      | p::rest => alt p (alts0 rest)
+    end.
+
+  Fixpoint half A (xs ys zs: list A) : (list A) * (list A) := 
+    match xs with 
+      | nil => (ys,zs) 
+      | h::t => half t zs (h::ys)
+    end.
+
+  Fixpoint alts' n t (ps:list (grammar t)) : grammar t := 
+    match n, ps with 
+      | 0%nat, _ => alts0 ps
+      | S n, nil => @never t
+      | S n, p::nil => p
+      | S n, ps => 
+        let (ps1,ps2) := half ps nil nil in 
+          let g1 := alts' n ps1 in 
+            let g2 := alts' n ps2 in 
+              alt g1 g2
+    end.
+
+  Definition alts t (ps:list (grammar t)) : grammar t := alts' 20 ps.
+
+
+Definition a0 := (prefix0 $ alts p0) @ (fun p => app (fst p) (snd p) %% listint_t).
+Definition a1 := (prefix1 $ alts p1) @ (fun p => app (fst p) (snd p) %% listint_t).
+Definition a2 := (prefix2 $ alts p2) @ (fun p => app (fst p) (snd p) %% listint_t).
+Definition a3 := (prefix3 $ alts p3) @ (fun p => app (fst p) (snd p) %% listint_t).
+Definition a4 := (prefix4 $ alts p4) @ (fun p => app (fst p) (snd p) %% listint_t).
+Definition a5 := (prefix5 $ alts p5) @ (fun p => app (fst p) (snd p) %% listint_t).
+Definition a6 := (prefix6 $ alts p6) @ (fun p => app (fst p) (snd p) %% listint_t).
+Definition a7 := (prefix7 $ alts p7) @ (fun p => app (fst p) (snd p) %% listint_t).
+Definition a8 := (prefix8 $ alts p8) @ (fun p => app (fst p) (snd p) %% listint_t).
+Definition a9 := (prefix9 $ alts p9) @ (fun p => app (fst p) (snd p) %% listint_t).
+Definition a10 := (prefix10 $ alts p10) @ (fun p => app (fst p) (snd p) %% listint_t).
+Definition a11 := (prefix11 $ alts p11) @ (fun p => app (fst p) (snd p) %% listint_t).
+Definition a12 := (prefix12 $ alts p12) @ (fun p => app (fst p) (snd p) %% listint_t).
+Definition a13 := (prefix13 $ alts p13) @ (fun p => app (fst p) (snd p) %% listint_t).
+
+End Grammar1.
+
+
+
+
+
+
+
+
+(* Module TEST_PARSER_ARG. *)
+(*   Definition char_p := bool. *)
+(*   Definition char_eq := Bool.bool_dec. *)
+
+(*   Inductive type : Set :=  *)
+(*   | Int_t : type. *)
+
+(*   Definition tipe := type. *)
+(*   Definition tipe_eq : forall (t1 t2:tipe), {t1=t2} + {t1<>t2}. *)
+(*     intros ; decide equality. *)
+(*   Defined. *)
+(*   Definition tipe_m (t:tipe) :=  *)
+(*     match t with  *)
+(*       | Int_t => nat *)
+(*     end. *)
+(* End TEST_PARSER_ARG. *)
+
+(* Module TEST_PARSER. *)
+(* Module T := Parser.Parser(TEST_PARSER_ARG). *)
+(* Import TEST_PARSER_ARG. *)
+(* Import T. *)
+(* Infix "|+|" := Alt_p (right associativity, at level 80). *)
+(* Infix "$" := Cat_p (right associativity, at level 70). *)
+(* Definition map_p t1 t2 (p:parser t1) (f:result_m t1 -> result_m t2) := @Map_p t1 t2 f p. *)
+(* Implicit Arguments map_p [t1 t2]. *)
+(* Infix "@" := map_p (right associativity, at level 75). *)
+(* Definition Plus_p t (p:parser t) :=  *)
+(*   (Cat_p p (Star_p p)) @ (fun p => ((fst p)::(snd p)): result_m (list_t t)). *)
+(* Definition Alts_p t (ps:list (parser t)) :=  *)
+(*   List.fold_right (@Alt_p t) (Zero_p t) ps. *)
+(* Definition int_t := tipe_t Int_t. *)
+(* Notation "e %% t" := (e : result_m t) (at level 80). *)
+
+(* Definition one := Char_p true @ (fun _ => 1 %% int_t). *)
+(* Definition zero := Char_p false @ (fun _ => 0 %% int_t). *)
+(* Definition bit' := zero |+| one. *)
+(* Definition bit := Any_p @ (fun c => (if c then 1 else 0) %% int_t). *)
+(* Definition nibble :=  *)
+(*   bit $ bit $ bit $ bit @  *)
+(*   (fun x => match x with  *)
+(*               | (b3,(b2,(b1,b0))) => b0 + 2*b1 + 4*b2 + 8*b3 *)
+(*             end %% int_t). *)
+(* Definition byte :=  *)
+(*   nibble $ nibble @ (fun p => (snd p + (fst p)*256) %% int_t). *)
+
+(* (* is a parser deterministic for strings up to length n?  *)
+(* Definition is_deterministic t (p:parser t) n :=  *)
+(*   is_determ (snd (parser2regexp p)) 2 (fun n => (match n with 0 => false | _ => true end)::nil) n *)
+(*   (fst (parser2regexp p)) (p2r_wf p _). *)
+
+(* Lemma is_deterministic_byte : is_deterministic byte 8 = true. *)
+(* Proof. *)
+(*   auto. *)
+(* Qed. *)
+
+(* Definition ambiguous_p := nibble |+| nibble. *)
+
+(* Lemma is_deterministic_ambiguous_p : is_deterministic ambiguous_p 4 = false. *)
+(* Proof. *)
+(*   auto. *)
+(* Qed. *)
+(* *) *)
+(* Fixpoint explode(s:string) : list bool :=  *)
+(*   match s with  *)
+(*     | ""%string => nil *)
+(*     | String "0" t => false::(explode t) *)
+(*     | String _ t => true::(explode t) *)
+(*   end. *)
+
+(* Definition lex t (p:parser t) s := parse p (explode s). *)
+
+(* (* *)
+(* Opaque result_m. *)
+(* Opaque p2r_wf. *)
+(* Opaque wf_derivs. *)
+(* *) *)
+(* Eval simpl in lex (nibble) "011".  *)
+(* Eval simpl in explode("1000111"). *)
+(* Eval simpl in nibble 1. *)
+(* End TEST_PARSER. *)
 
   
 
